concrete/exec.v
@@ -1,10 +1,9 @@
 (* Executable formulation of concrete machine semantics *)
 
-Require Import ZArith.
-Require Import ssreflect ssrfun ssrbool eqtype ssrnat.
+Require Import ssreflect ssrfun ssrbool eqtype ssrnat ssrint.
+Require Import word partmap.
 Require Import lib.utils common.common concrete.concrete.
 
-Import ListNotations.
 Import Concrete. Import DoNotation.
 
 Set Implicit Arguments.
@@ -22,59 +21,59 @@ Context {ops : machine_ops mt}.
 
 Open Scope word_scope.
 
-Local Notation "x .+1" := (x + Word.one).
+Local Notation "x .+1" := (x + 1).
 
 (* TODO: mt should be named t, or vice versa, globally! *)
 Definition step (st : state mt) : option (state mt) :=
   let 'mkState mem reg cache pc@tpc epc := st in
-  do! i <- PartMaps.get mem pc;
+  do! i <- mem pc;
   do! instr <- decode_instr (val i);
-  let mvec := mkMVec (op_to_word (opcode_of instr)) tpc (tag i) in
+  let mvec := mkMVec (mword_of_op (opcode_of instr)) tpc (tag i) in
   match instr with
   | Nop =>
     let mvec := mvec TNone TNone TNone in
     next_state_pc masks st mvec (pc.+1)
   | Const n r =>
-    do! old <- PartMaps.get reg r;
+    do! old <- reg r;
     let mvec := mvec (tag old) TNone TNone in
-    next_state_reg masks st mvec r (Word.casts n)
+    next_state_reg masks st mvec r (swcast n)
   | Mov r1 r2 =>
-    do! v1 <- PartMaps.get reg r1;
-    do! old <- PartMaps.get reg r2;
+    do! v1 <- reg r1;
+    do! old <- reg r2;
     let mvec := mvec (tag v1) (tag old) TNone in
     next_state_reg masks st mvec r2 (val v1)
   | Binop f r1 r2 r3 =>
-    do! v1 <- PartMaps.get reg r1;
-    do! v2 <- PartMaps.get reg r2;
-    do! old <- PartMaps.get reg r3;
+    do! v1 <- reg r1;
+    do! v2 <- reg r2;
+    do! old <- reg r3;
     let mvec := mvec (tag v1) (tag v2) (tag old) in
     next_state_reg masks st mvec r3 (binop_denote f (val v1) (val v2))
   | Load r1 r2 =>
-    do! v1 <- PartMaps.get reg r1;
-    do! v2 <- PartMaps.get mem (val v1);
-    do! old <- PartMaps.get reg r2;
+    do! v1 <- reg r1;
+    do! v2 <- mem (val v1);
+    do! old <- reg r2;
     let mvec := mvec (tag v1) (tag v2) (tag old) in
     next_state_reg masks st mvec r2 (val v2)
   | Store r1 r2 =>
-    do! v1 <- PartMaps.get reg r1;
-    do! v2 <- PartMaps.get reg r2;
-    do! v3 <- PartMaps.get mem (val v1);
+    do! v1 <- reg r1;
+    do! v2 <- reg r2;
+    do! v3 <- mem (val v1);
     let mvec := mvec (tag v1) (tag v2) (tag v3) in
     next_state masks st mvec (fun rvec =>
-      do! mem' <- PartMaps.upd mem (val v1) (val v2)@(ctr rvec);
+      do! mem' <- updm mem (val v1) (val v2)@(ctr rvec);
       Some (mkState mem' reg cache (pc.+1)@(ctrpc rvec) epc))
   | Jump r =>
-    do! v <- PartMaps.get reg r;
+    do! v <- reg r;
     let mvec := mvec (tag v) TNone TNone in
     next_state_pc masks st mvec (val v)
   | Bnz r n =>
-    do! v <- PartMaps.get reg r;
+    do! v <- reg r;
     let mvec := mvec (tag v) TNone TNone in
-    let pc' := pc + if (val v) == Word.zero then Word.one else Word.casts n in
+    let pc' := pc + if (val v) == 0%w then 1%w else swcast n in
     next_state_pc masks st mvec pc'
   | Jal r =>
-    do! v <- PartMaps.get reg r;
-    do! old <- PartMaps.get reg ra;
+    do! v <- reg r;
+    do! old <- reg ra;
     let mvec := mvec (tag v) (tag old) TNone in
     next_state_reg_and_pc masks st mvec ra (pc.+1) (val v)
   | JumpEpc =>
@@ -86,17 +85,17 @@ Definition step (st : state mt) : option (state mt) :=
       do! cache' <- add_rule cache masks mem;
       Some (mkState mem reg cache' (pc.+1)@(ctrpc rvec) epc))
   | GetTag r1 r2 =>
-    do! v1 <- PartMaps.get reg r1;
-    do! old <- PartMaps.get reg r2;
+    do! v1 <- reg r1;
+    do! old <- reg r2;
     let mvec := mvec (tag v1) (tag old) TNone in
     next_state_reg masks st mvec r2 (tag v1)
   | PutTag r1 r2 r3 =>
-    do! v1 <- PartMaps.get reg r1;
-    do! v2 <- PartMaps.get reg r2;
-    do! old <- PartMaps.get reg r3;
+    do! v1 <- reg r1;
+    do! v2 <- reg r2;
+    do! old <- reg r3;
     let mvec := mvec (tag v1) (tag v2) (tag old) in
     next_state masks st mvec (fun rvec =>
-      do! reg' <- PartMaps.upd reg r3 (val v1)@(val v2);
+      do! reg' <- updm reg r3 (val v1)@(val v2);
       Some (mkState mem reg' cache (pc.+1)@(ctrpc rvec) epc))
   | Halt => None
 end.
@@ -145,56 +144,54 @@ Proof.
     + rewrite M1. simpl. trivial.
 Qed.
 
-Lemma stepP' : forall s1 s2, ssrbool.reflect (Concrete.step _ masks s1 s2) (step s1 == Some s2).
+Lemma stepP' : forall s1 s2, reflect (Concrete.step _ masks s1 s2) (step s1 == Some s2).
 Proof.
   move => s1 s2.
   apply (iffP eqP); by move => /stepP.
 Qed.
 
-Import PartMaps.
-
-Definition build_cmvec st : option (Concrete.MVec (word mt)) :=
-  match get (Concrete.mem st) (Concrete.pcv st) with
+Definition build_cmvec st : option (Concrete.MVec (mword mt)) :=
+  match Concrete.mem st (Concrete.pcv st) with
     | Some i =>
       match decode_instr (val i) with
         | Some op =>
-          let part := @Concrete.mkMVec (word mt) (op_to_word (opcode_of op))
+          let part := @Concrete.mkMVec (mword mt) (mword_of_op (opcode_of op))
                                        (Concrete.pct st) (common.tag i) in
           match op  with
             | Nop => fun part => Some (part Concrete.TNone Concrete.TNone Concrete.TNone)
             | Const n r =>
               fun part =>
-                do! old <- PartMaps.get (Concrete.regs st) r;
+                do! old <- (Concrete.regs st) r;
                   Some (part (common.tag old) Concrete.TNone Concrete.TNone)
             | Mov r1 r2 =>
               fun part =>
-                do! v1 <- PartMaps.get (Concrete.regs st) r1;
-                do! v2 <- PartMaps.get (Concrete.regs st) r2;
+                do! v1 <- (Concrete.regs st) r1;
+                do! v2 <- (Concrete.regs st) r2;
                   Some (part (common.tag v1) (common.tag v2) Concrete.TNone)
             | Binop _ r1 r2 r3 => fun part =>
-              do! v1 <- PartMaps.get (Concrete.regs st) r1;
-              do! v2 <- PartMaps.get (Concrete.regs st) r2;
-              do! v3 <- PartMaps.get (Concrete.regs st) r3;
+              do! v1 <- (Concrete.regs st) r1;
+              do! v2 <- (Concrete.regs st) r2;
+              do! v3 <- (Concrete.regs st) r3;
                 Some (part (common.tag v1) (common.tag v2) (common.tag v3))
             | Load r1 r2 => fun part =>
-              do! w1 <- PartMaps.get (Concrete.regs st) r1;
-              do! w2 <- get (Concrete.mem st) (val w1);
-              do! old <- PartMaps.get (Concrete.regs st) r2;
+              do! w1 <- (Concrete.regs st) r1;
+              do! w2 <- Concrete.mem st (val w1);
+              do! old <- (Concrete.regs st) r2;
                 Some (part (common.tag w1) (common.tag w2) (common.tag old))
             | Store r1 r2 => fun part =>
-              do! w1 <- PartMaps.get (Concrete.regs st) r1;
-              do! w2 <- PartMaps.get (Concrete.regs st) r2;
-                do! w3 <- get (Concrete.mem st) (val w1);
+              do! w1 <- (Concrete.regs st) r1;
+              do! w2 <- (Concrete.regs st) r2;
+                do! w3 <- Concrete.mem st (val w1);
                 Some (part (common.tag w1) (common.tag w2) (common.tag w3))
             | Jump r => fun part =>
-              do! w <- PartMaps.get (Concrete.regs st) r;
+              do! w <- (Concrete.regs st) r;
                 Some (part (common.tag w) Concrete.TNone Concrete.TNone)
             | Bnz r n => fun part =>
-              do! w <- PartMaps.get (Concrete.regs st) r;
+              do! w <- (Concrete.regs st) r;
                 Some (part (common.tag w) Concrete.TNone Concrete.TNone)
             | Jal r => fun part =>
-              do! w <- PartMaps.get (Concrete.regs st) r;
-              do! old <- PartMaps.get (Concrete.regs st) ra;
+              do! w <- (Concrete.regs st) r;
+              do! old <- (Concrete.regs st) ra;
                 Some (part (common.tag w) (common.tag old) Concrete.TNone)
             | JumpEpc =>
               fun part =>
@@ -204,14 +201,14 @@ Definition build_cmvec st : option (Concrete.MVec (word mt)) :=
                 Some (part Concrete.TNone Concrete.TNone Concrete.TNone)
             | GetTag r1 r2 =>
               fun part =>
-                do! w1 <- PartMaps.get (Concrete.regs st) r1;
-                do! old <- PartMaps.get (Concrete.regs st) r2;
+                do! w1 <- (Concrete.regs st) r1;
+                do! old <- (Concrete.regs st) r2;
                 Some (part (common.tag w1) (common.tag old) Concrete.TNone)
             | PutTag r1 r2 r3 =>
               fun part =>
-                do! w1 <- PartMaps.get (Concrete.regs st) r1;
-                do! w2 <- PartMaps.get (Concrete.regs st) r2;
-                do! old <- PartMaps.get (Concrete.regs st) r3;
+                do! w1 <- (Concrete.regs st) r1;
+                do! w2 <- (Concrete.regs st) r2;
+                do! old <- (Concrete.regs st) r3;
                 Some (part (common.tag w1) (common.tag w2) (common.tag old))
             | Halt => fun _ => None
           end part
@@ -227,15 +224,12 @@ Lemma step_lookup_success_or_fault cst cst' :
     match cache_lookup (cache cst) masks cmvec with
     | Some crvec => pct cst' = ctrpc crvec
     | None =>
-      match store_mvec (mem cst) cmvec with
-      | Some cmem' =>
-        cst' = mkState cmem'
-                       (regs cst)
-                       (cache cst)
-                       (fault_handler_start mt)@TKernel
-                       (pc cst)
-      | None => False
-      end
+      let cmem' := store_mvec (mem cst) cmvec in
+      cst' = mkState cmem'
+                     (regs cst)
+                     (cache cst)
+                     (fault_handler_start mt)@TKernel
+                     (pc cst)
     end.
 Proof.
   move => STEP.
@@ -254,7 +248,7 @@ Qed.
 Lemma lookup_none_step cst cmvec cmem :
   build_cmvec cst = Some cmvec ->
   Concrete.cache_lookup (Concrete.cache cst) masks cmvec = None ->
-  Concrete.store_mvec (Concrete.mem cst) cmvec = Some cmem ->
+  Concrete.store_mvec (Concrete.mem cst) cmvec = cmem ->
   Concrete.step _ masks cst (Concrete.mkState cmem
                                               (Concrete.regs cst)
                                               (Concrete.cache cst)
@@ -266,11 +260,11 @@ Proof.
   rewrite (Concrete.state_eta cst) /=.
   move: CMVEC.
   rewrite /build_cmvec.
-  case: (get _ _) => [[i ti]|] //=.
+  case: (getm _ _) => [[i ti]|] //=.
   case: (decode_instr i) => [instr|] //= CMVEC;
   destruct instr; simpl in *; match_inv;
   by rewrite /next_state_reg /next_state_pc /next_state_reg_and_pc /next_state /miss_state //=
-             LOOKUP STORE.
+             LOOKUP.
 Qed.
 
 Lemma step_build_cmvec cst cst' :
@@ -300,13 +294,13 @@ Qed.
 Lemma build_cmvec_cop_cti cst cmvec :
   build_cmvec cst = Some cmvec ->
   exists i instr,
-    [/\ PartMaps.get (Concrete.mem cst) (Concrete.pcv cst) =
+    [/\ (Concrete.mem cst) (Concrete.pcv cst) =
         Some i@(Concrete.cti cmvec),
         decode_instr i = Some instr &
-        op_to_word (opcode_of instr) = Concrete.cop cmvec].
+        mword_of_op (opcode_of instr) = Concrete.cop cmvec].
 Proof.
   rewrite /build_cmvec.
-  case: (get _ _) => [[i ti]|] //= MVEC. exists i. move: MVEC.
+  case: (getm _ _) => [[i ti]|] //= MVEC. exists i. move: MVEC.
   case: (decode_instr i) => [instr|] //= MVEC. exists instr.
   destruct instr; match_inv; simpl; eauto using And3.
   discriminate.
