sealing/abstract.v
@@ -1,13 +1,8 @@
-Require Import List. Import ListNotations.
-Require Import Coq.Bool.Bool.
-Require Import Coq.Classes.SetoidDec.
 Require Import ssreflect ssrfun ssrbool eqtype seq.
-Require Import lib.utils.
+Require Import word partmap.
+Require Import lib.utils common.common sealing.classes.
 
 Import DoNotation.
-
-Require Import lib.utils common.common.
-Require Import sealing.classes.
 
 Set Implicit Arguments.
 Unset Strict Implicit.
@@ -35,32 +30,30 @@ Class sealing_key := {
 Context {sk : sealing_key}.
 
 Inductive value :=
-| VData   : word t        -> value
-| VKey    :           key -> value
-| VSealed : word t -> key -> value.
+| VData   : mword t        -> value
+| VKey    :            key -> value
+| VSealed : mword t -> key -> value.
 
-Import PartMaps.
-
-Local Notation memory := (word_map t value).
-Local Notation registers := (reg_map t value).
+Local Notation memory := {partmap mword t -> value}.
+Local Notation registers := {partmap reg t -> value}.
 
 Open Scope word_scope.
 
-Local Notation "x .+1" := (Word.add x Word.one) (at level 60).
+Local Notation "x .+1" := (x + 1) (at level 60).
 
 Record state := State {
   mem : memory;
   regs : registers;
-  pc : word t;
-  keys : list key
+  pc : mword t;
+  keys : seq key
 }.
 
-Definition syscall_addrs := [mkkey_addr; seal_addr; unseal_addr].
+Definition syscall_addrs := [:: mkkey_addr; seal_addr; unseal_addr].
 
 Notation "x '=?' y" := (x = Some y) (at level 99).
 
-Definition decode (mem : memory) (pc : word t) :=
-  match get mem pc with
+Definition decode (mem : memory) (pc : mword t) :=
+  match mem pc with
     | Some (VData i) => decode_instr i
     | _              => None
   end.
@@ -73,74 +66,74 @@ Inductive step (st st' : state) : Prop :=
 | step_const : forall mem reg reg' pc n r ks
     (ST   : st = State mem reg pc ks)
     (INST : decode mem pc =? Const n r)
-    (UPD  : upd reg r (VData (Word.casts n)) =? reg')
+    (UPD  : updm reg r (VData (swcast n)) =? reg')
     (NEXT : st' = State mem reg' (pc.+1) ks),   step st st'
 | step_mov : forall mem reg reg' pc r1 v1 r2 ks
     (ST   : st = State mem reg pc ks)
     (INST : decode mem pc =? Mov r1 r2)
-    (R1W  : get reg r1 =? v1)
-    (UPD  : upd reg r2 v1 =? reg')
+    (R1W  : reg r1 =? v1)
+    (UPD  : updm reg r2 v1 =? reg')
     (NEXT : st' = State mem reg' (pc.+1) ks),   step st st'
 | step_binop : forall mem reg reg' pc op r1 r2 r3 w1 w2 ks
     (ST   : st = State mem reg pc ks)
     (INST : decode mem pc =? Binop op r1 r2 r3)
-    (R1W  : get reg r1 =? VData w1)
-    (R2W  : get reg r2 =? VData w2)
-    (UPD  : upd reg r3 (VData (binop_denote op w1 w2)) =? reg')
+    (R1W  : reg r1 =? VData w1)
+    (R2W  : reg r2 =? VData w2)
+    (UPD  : updm reg r3 (VData (binop_denote op w1 w2)) =? reg')
     (NEXT : st' = State mem reg' (pc.+1) ks),   step st st'
 | step_load : forall mem reg reg' pc r1 r2 w1 v2 ks
     (ST   : st = State mem reg pc ks)
     (INST : decode mem pc =? Load r1 r2)
-    (R1W  : get reg r1 =? VData w1)
-    (MEM1 : get mem w1 =? v2)
-    (UPD  : upd reg r2 v2 =? reg')
+    (R1W  : reg r1 =? VData w1)
+    (MEM1 : mem w1 =? v2)
+    (UPD  : updm reg r2 v2 =? reg')
     (NEXT : st' = State mem reg' (pc.+1) ks),   step st st'
 | step_store : forall mem mem' reg pc r1 r2 w1 v2 ks
     (ST   : st = State mem reg pc ks)
     (INST : decode mem pc =? Store r1 r2)
-    (R1W  : get reg r1 =? VData w1)
-    (R2W  : get reg r2 =? v2)
-    (UPDM : upd mem w1 v2 =? mem')
+    (R1W  : reg r1 =? VData w1)
+    (R2W  : reg r2 =? v2)
+    (UPDM : updm mem w1 v2 =? mem')
     (NEXT : st' = State mem' reg (pc.+1) ks),   step st st'
 | step_jump : forall mem reg pc r w ks
     (ST   : st = State mem reg pc ks)
     (INST : decode mem pc =? Jump r)
-    (RW   : get reg r =? VData w)
+    (RW   : reg r =? VData w)
     (NEXT : st' = State mem reg w ks),   step st st'
 | step_bnz : forall mem reg pc r n w ks
     (ST   : st = State mem reg pc ks)
     (INST : decode mem pc =? Bnz r n)
-    (RW   : get reg r =? VData w),
-    let pc' := Word.add pc (if w == Word.zero
-                            then Word.one else Word.casts n) in forall
+    (RW   : reg r =? VData w),
+    let pc' := pc + (if w == 0
+                     then 1 else swcast n) in forall
     (NEXT : st' = State mem reg pc' ks),   step st st'
 | step_jal : forall mem reg reg' pc r w ks
     (ST   : st = State mem reg pc ks)
     (INST : decode mem pc =? Jal r)
-    (RW   : get reg r =? VData w)
-    (UPD  : upd reg ra (VData (pc.+1)) =? reg')
+    (RW   : reg r =? VData w)
+    (UPD  : updm reg ra (VData (pc.+1)) =? reg')
     (NEXT : st' = State mem reg' w ks),   step st st'
 | step_mkkey : forall mem reg reg' pc ks
     (ST   : st = State mem reg mkkey_addr ks)
     (INST : decode mem mkkey_addr = None)
-    (UPD  : upd reg syscall_ret (VKey (mkkey_f ks)) =? reg')
-    (RET  : get reg ra =? VData pc)
+    (UPD  : updm reg syscall_ret (VKey (mkkey_f ks)) =? reg')
+    (RET  : reg ra =? VData pc)
     (NEXT : st' = State mem reg' pc ((mkkey_f ks) :: ks)),   step st st'
 | step_seal : forall mem reg reg' pc ks payload key
     (ST   : st = State mem reg seal_addr ks)
     (INST : decode mem seal_addr = None)
-    (R1   : get reg syscall_arg1 =? VData payload)
-    (R2   : get reg syscall_arg2 =? VKey key)
-    (UPD  : upd reg syscall_ret (VSealed payload key) =? reg')
-    (RET  : get reg ra =? VData pc)
+    (R1   : reg syscall_arg1 =? VData payload)
+    (R2   : reg syscall_arg2 =? VKey key)
+    (UPD  : updm reg syscall_ret (VSealed payload key) =? reg')
+    (RET  : reg ra =? VData pc)
     (NEXT : st' = State mem reg' pc ks),   step st st'
 | step_unseal : forall mem reg reg' pc ks payload key
     (ST   : st = State mem reg unseal_addr ks)
     (INST : decode mem unseal_addr = None)
-    (R1   : get reg syscall_arg1 =? VSealed payload key)
-    (R2   : get reg syscall_arg2 =? VKey key)
-    (UPD  : upd reg syscall_ret (VData payload) =? reg')
-    (RET  : get reg ra =? VData pc)
+    (R1   : reg syscall_arg1 =? VSealed payload key)
+    (R2   : reg syscall_arg2 =? VKey key)
+    (UPD  : updm reg syscall_ret (VData payload) =? reg')
+    (RET  : reg ra =? VData pc)
     (NEXT : st' = State mem reg' pc ks),   step st st'.
 
 Definition stepf (st : state) : option state :=
@@ -149,49 +142,49 @@ Definition stepf (st : state) : option state :=
     | Some Nop =>
       Some (State mem reg (pc.+1) keys)
     | Some (Const n r) =>
-      do! reg' <- PartMaps.upd reg r (VData (Word.casts n));
+      do! reg' <- updm reg r (VData (swcast n));
       Some (State mem reg' (pc.+1) keys)
     | Some (Mov r1 r2) =>
-      do! v <- PartMaps.get reg r1;
-      do! reg' <- PartMaps.upd reg r2 v;
+      do! v <- reg r1;
+      do! reg' <- updm reg r2 v;
       Some (State mem reg' (pc.+1) keys)
     | Some (Binop b r1 r2 r3) =>
-      do! v1 <- PartMaps.get reg r1;
-      do! v2 <- PartMaps.get reg r2;
+      do! v1 <- reg r1;
+      do! v2 <- reg r2;
       if v1 is VData i1 then if v2 is VData i2 then
-        do! reg' <- PartMaps.upd reg r3 (VData (binop_denote b i1 i2));
+        do! reg' <- updm reg r3 (VData (binop_denote b i1 i2));
         Some (State mem reg' (pc.+1) keys)
       else None else None
     | Some (Load r1 r2) =>
-      do! v <- PartMaps.get reg r1;
+      do! v <- reg r1;
       if v is VData i then
-        do! v' <- PartMaps.get mem i;
-        do! reg' <- PartMaps.upd reg r2 v';
+        do! v' <- mem i;
+        do! reg' <- updm reg r2 v';
         Some (State mem reg' (pc.+1) keys)
       else None
     | Some (Store r1 r2) =>
-      do! v1 <- PartMaps.get reg r1;
-      do! v2 <- PartMaps.get reg r2;
+      do! v1 <- reg r1;
+      do! v2 <- reg r2;
       if v1 is VData i1 then
-        do! mem' <- PartMaps.upd mem i1 v2;
+        do! mem' <- updm mem i1 v2;
         Some (State mem' reg (pc.+1) keys)
       else None
     | Some (Jump r) =>
-      do! v <- PartMaps.get reg r;
+      do! v <- reg r;
       if v is VData i then
         Some (State mem reg i keys)
       else None
     | Some (Bnz r n) =>
-      do! vr <- PartMaps.get reg r;
+      do! vr <- reg r;
       if vr is VData c then
-        let pc' := pc + if c == Word.zero
-                        then Word.one else Word.casts n in
+        let pc' := pc + if c == 0
+                        then 1 else swcast n in
         Some (State mem reg pc' keys)
       else None
     | Some (Jal r) =>
-      do! vr <- PartMaps.get reg r;
+      do! vr <- reg r;
       if vr is VData i then
-        do! reg' <- PartMaps.upd reg ra (VData (pc.+1));
+        do! reg' <- updm reg ra (VData (pc.+1));
         Some (State mem reg' i keys)
       else None
     | Some JumpEpc | Some AddRule | Some (GetTag _ _)
@@ -201,28 +194,28 @@ Definition stepf (st : state) : option state :=
     if pc == mkkey_addr then
       let k := mkkey_f keys in
       let keys' := k :: keys in
-      do! reg' <- PartMaps.upd reg syscall_ret (VKey k);
-      do! ret <- PartMaps.get reg ra;
+      do! reg' <- updm reg syscall_ret (VKey k);
+      do! ret <- reg ra;
       if ret is VData pc' then
         Some (State mem reg' pc' keys')
       else None
     else if pc == seal_addr then
-      do! v1 <- PartMaps.get reg syscall_arg1;
-      do! v2 <- PartMaps.get reg syscall_arg2;
+      do! v1 <- reg syscall_arg1;
+      do! v2 <- reg syscall_arg2;
       if v1 is VData payload then if v2 is VKey k then
-        do! reg' <- PartMaps.upd reg syscall_ret (VSealed payload k);
-        do! ret <- PartMaps.get reg ra;
+        do! reg' <- updm reg syscall_ret (VSealed payload k);
+        do! ret <- reg ra;
         if ret is VData pc' then
           Some (State mem reg' pc' keys)
         else None
       else None else None
     else if pc == unseal_addr then
-      do! v1 <- PartMaps.get reg syscall_arg1;
-      do! v2 <- PartMaps.get reg syscall_arg2;
+      do! v1 <- reg syscall_arg1;
+      do! v2 <- reg syscall_arg2;
       if v1 is VSealed payload k then if v2 is VKey k' then
         if k == k' then
-          do! reg' <- PartMaps.upd reg syscall_ret (VData payload);
-          do! ret <- PartMaps.get reg ra;
+          do! reg' <- updm reg syscall_ret (VData payload);
+          do! ret <- reg ra;
           if ret is VData pc' then
             Some (State mem reg' pc' keys)
           else None
@@ -239,34 +232,34 @@ Definition stepf (st : state) : option state :=
 
 Program Definition abstract_initial_state
       (user_mem : relocatable_segment classes.sealing_syscall_addrs value)
-      (base_addr : word t)
-      (user_regs : list (reg t))
+      (base_addr : mword t)
+      (user_regs : seq (reg t))
     : state :=
   let (_, gen) := user_mem in
   let mem_contents := gen base_addr ssa in
   let mem :=
-    snd (fold_left
+    snd (foldl
       (fun x c => let: (i,m) := x in
-                  (Word.add Word.one i, PartMaps.set m i c))
-      mem_contents
-      (base_addr, PartMaps.empty))
+                  (1 + i, setm m i c))
+      (base_addr, emptym)
+      mem_contents)
+
       in
   let regs :=
-        fold_left
-          (fun regs r => PartMaps.set regs r (VData Word.zero))
-           user_regs
-           PartMaps.empty in
+        foldl
+          (fun regs r => setm regs r (VData 0))
+           emptym user_regs in
   {|
     mem := mem;
     regs := regs;
     pc := base_addr;
-    keys := []
+    keys := [::]
   |}.
 
 End WithClasses.
 
-Notation memory t := (word_map t (@value t _)).
-Notation registers t := (reg_map t (@value t _)).
+Notation memory t := {partmap mword t -> @value t _}.
+Notation registers t := {partmap reg t -> @value t _}.
 
 End Abs.
 
