symbolic/refinement_common.v
@@ -1,6 +1,5 @@
-Require Import NPeano Arith Bool.
-
 Require Import ssreflect ssrfun ssrbool eqtype ssrnat seq.
+Require Import hseq word partmap.
 
 Require Import lib.utils.
 Require Import common.common.
@@ -9,8 +8,6 @@ Require Import concrete.exec.
 Require Import symbolic.symbolic.
 Require Import symbolic.exec.
 Require Import symbolic.rules.
-
-Open Scope nat_scope.
 
 Set Implicit Arguments.
 Unset Strict Implicit.
@@ -31,26 +28,26 @@ Context {mt : machine_types}
 Definition refine_memory (amem : Symbolic.memory mt _) (cmem : Concrete.memory mt) :=
   (forall w x ctg atg,
      decode Symbolic.M cmem ctg = Some (USER atg) ->
-     PartMaps.get cmem w = Some x@ctg ->
-     PartMaps.get amem w = Some x@atg) /\
+     cmem w = Some x@ctg ->
+     amem w = Some x@atg) /\
   (forall w x atg,
-     PartMaps.get amem w = Some x@atg ->
+     amem w = Some x@atg ->
      exists2 ctg,
        decode Symbolic.M cmem ctg = Some (USER atg) &
-       PartMaps.get cmem w = Some x@ctg).
+       cmem w = Some x@ctg).
 
 Definition refine_registers (areg : Symbolic.registers mt _)
                             (creg : Concrete.registers mt)
                             (cmem : Concrete.memory mt) :=
   (forall r x ctg atg,
      decode Symbolic.R cmem ctg = Some (USER atg) ->
-     PartMaps.get creg r = Some x@ctg ->
-     PartMaps.get areg r = Some x@atg) /\
+     creg r = Some x@ctg ->
+     areg r = Some x@atg) /\
   (forall r x atg,
-     PartMaps.get areg r = Some x@atg ->
+     areg r = Some x@atg ->
      exists2 ctg,
        decode Symbolic.R cmem ctg = Some (USER atg) &
-       PartMaps.get creg r = Some x@ctg).
+       creg r = Some x@ctg).
 
 Definition in_kernel (st : Concrete.state mt) :=
   Concrete.is_kernel_tag (Concrete.pct st).
@@ -69,41 +66,25 @@ Definition cache_correct cache cmem :=
           decode_ovec e (Symbolic.op ivec) cmem crvec = Some ovec &
           Symbolic.transfer ivec = Some ovec ].
 
-Definition in_mvec addr := In addr (Concrete.mvec_fields mt).
+Definition in_mvec addr := addr \in Concrete.mvec_fields mt.
 
 Definition mvec_in_kernel (cmem : Concrete.memory mt) :=
   forall addr,
     in_mvec addr ->
-    exists w : (word mt), PartMaps.get cmem addr = Some w@Concrete.TKernel.
+    exists w : mword mt, cmem addr = Some w@Concrete.TKernel.
 
 Lemma store_mvec_mvec_in_kernel cmem cmem' mvec :
-  Concrete.store_mvec cmem mvec = Some cmem' ->
+  Concrete.store_mvec cmem mvec = cmem' ->
   mvec_in_kernel cmem'.
 Proof.
-  unfold Concrete.store_mvec, mvec_in_kernel, in_mvec.
-  intros H addr IN.
-  destruct (PartMaps.get_upd_list_in H IN)
-    as (v' & IN' & GET).
-  rewrite GET.
-  simpl in IN'.
-  repeat match goal with
-  | H : _ \/ _ |- _ => destruct H as [E | ?]; [inv E|]
-  | H : False |- _ => destruct H
-  end; eauto.
-Qed.
-
-Lemma mvec_in_kernel_store_mvec cmem mvec :
-  mvec_in_kernel cmem ->
-  exists cmem',
-    Concrete.store_mvec cmem mvec = Some cmem'.
-Proof.
-  unfold mvec_in_kernel, in_mvec, Concrete.mvec_fields, Concrete.store_mvec.
-  intros DEF.
-  eapply PartMaps.upd_list_defined; eauto; try apply word_map_axioms.
-  simpl map. intros addr IN.
-  apply DEF in IN.
-  destruct IN.
-  eauto.
+move=> <- k; rewrite /Concrete.store_mvec getm_union.
+set m := mkpartmap _.
+rewrite -[isSome (m k)]/(k \in m) mem_mkpartmap /in_mvec /Concrete.mvec_fields.
+move=> E; rewrite E; have: k \in m by rewrite mem_mkpartmap.
+rewrite inE {E}; case E: (m k) => [v|] // _.
+move/getm_mkpartmap': E; rewrite !inE.
+do !(case/orP=> [/eqP [_ ->]|]; eauto).
+by move/eqP => [_ ->]; eauto.
 Qed.
 
 (* CH: kernel_invariant only holds when kernel starts executing, can
@@ -118,30 +99,30 @@ Qed.
 Record kernel_invariant : Type := {
   kernel_invariant_statement :> Concrete.memory mt ->
                                 Concrete.registers mt ->
-                                Concrete.rules (word mt) ->
+                                Concrete.rules (mword mt) ->
                                 Symbolic.internal_state -> Prop;
 
   kernel_invariant_upd_mem :
     forall regs mem1 mem2 cache addr w1 ct ut w2 int
            (KINV : kernel_invariant_statement mem1 regs cache int)
-           (GET : PartMaps.get mem1 addr = Some w1@ct)
+           (GET : mem1 addr = Some w1@ct)
            (DEC : decode Symbolic.M mem1 ct = Some (USER ut))
-           (UPD : PartMaps.upd mem1 addr w2 = Some mem2),
+           (UPD : updm mem1 addr w2 = Some mem2),
       kernel_invariant_statement mem2 regs cache int;
 
   kernel_invariant_upd_reg :
     forall mem regs1 regs2 cache r w1 ct1 ut1 w2 ct2 ut2 int
            (KINV : kernel_invariant_statement mem regs1 cache int)
-           (GET : PartMaps.get regs1 r = Some w1@ct1)
+           (GET : regs1 r = Some w1@ct1)
            (DEC1 : decode Symbolic.R mem ct1 = Some (USER ut1))
-           (UPD : PartMaps.upd regs1 r w2@ct2 = Some regs2)
+           (UPD : updm regs1 r w2@ct2 = Some regs2)
            (DEC2 : decode Symbolic.R mem ct2 = Some (USER ut2)),
       kernel_invariant_statement mem regs2 cache int;
 
   kernel_invariant_store_mvec :
     forall mem mem' mvec regs cache int
            (KINV : kernel_invariant_statement mem regs cache int)
-           (MVEC : Concrete.store_mvec mem mvec = Some mem'),
+           (MVEC : Concrete.store_mvec mem mvec = mem'),
       kernel_invariant_statement mem' regs cache int
 }.
 
@@ -162,7 +143,7 @@ Qed.
 
 Variable table : list (Symbolic.syscall mt).
 
-Definition is_nop (i : word mt) : bool :=
+Definition is_nop (i : mword mt) : bool :=
   match decode_instr i with
   | Some Nop => true
   | _ => false
@@ -179,7 +160,7 @@ Definition wf_entry_points (cmem : Concrete.memory mt) :=
   forall addr t,
     (exists2 sc, Symbolic.get_syscall table addr = Some sc &
                  Symbolic.entry_tag sc = t) <->
-    is_true match PartMaps.get cmem addr with
+    is_true match cmem addr with
             | Some i@it => is_nop i && (decode Symbolic.M cmem it == Some (ENTRY t))
             | None => false
             end.
@@ -188,7 +169,7 @@ Lemma wf_entry_points_if cmem addr sc :
   wf_entry_points cmem ->
   Symbolic.get_syscall table addr = Some sc ->
   exists i it,
-  [/\ PartMaps.get cmem addr = Some i@it,
+  [/\ cmem addr = Some i@it,
       decode Symbolic.M cmem it = Some (ENTRY (Symbolic.entry_tag sc)) &
       is_nop i ].
 Proof.
@@ -196,7 +177,7 @@ Proof.
   have: exists2 sc', Symbolic.get_syscall table addr = Some sc' &
                      Symbolic.entry_tag sc' = Symbolic.entry_tag sc by eauto.
   move/WFENTRYPOINTS.
-  case: (PartMaps.get cmem addr) => [[i it]|] //.
+  case: (cmem addr) => [[i it]|] //.
   move/andP => [H1 H2]. exists i, it.
   split; trivial.
   by apply/eqP.
@@ -204,7 +185,7 @@ Qed.
 
 Lemma wf_entry_points_only_if cmem addr i it t :
   wf_entry_points cmem ->
-  PartMaps.get cmem addr = Some i@it ->
+  cmem addr = Some i@it ->
   decode Symbolic.M cmem it = Some (ENTRY t) ->
   is_nop i ->
   exists2 sc,
@@ -213,17 +194,17 @@ Lemma wf_entry_points_only_if cmem addr i it t :
 Proof.
   move => WF GET DEC ISNOP.
   apply/WF.
-  by rewrite GET DEC eqxx andb_true_r.
+  by rewrite GET DEC eqxx andbT.
 Qed.
 
 Lemma entry_point_undefined cmem smem addr v it t :
   refine_memory smem cmem ->
-  PartMaps.get cmem addr = Some v@it ->
+  cmem addr = Some v@it ->
   decode Symbolic.M cmem it = Some (ENTRY t) ->
-  PartMaps.get smem addr = None.
+  smem addr = None.
 Proof.
   move => REFM GET DEC.
-  case GET': (PartMaps.get smem addr) => [[v' t']|] //.
+  case GET': (smem addr) => [[v' t']|] //.
   move/(proj2 REFM): GET'.
   rewrite GET. case=> it' H1 [? ?]. subst v' it'. congruence.
 Qed.
@@ -253,28 +234,28 @@ Lemma refine_memory_upd cache aregs cregs amem cmem cmem' addr v v' ct t ct' t' 
   cache_correct cache cmem ->
   refine_registers aregs cregs cmem ->
   refine_memory amem cmem ->
-  PartMaps.get cmem addr = Some v@ct ->
+  cmem addr = Some v@ct ->
   decode Symbolic.M cmem ct = Some (USER t) ->
-  PartMaps.upd cmem addr v'@ct' = Some cmem' ->
+  updm cmem addr v'@ct' = Some cmem' ->
   decode Symbolic.M cmem ct' = Some (USER t') ->
   exists amem',
-    [/\ PartMaps.upd amem addr v'@t' = Some amem',
+    [/\ updm amem addr v'@t' = Some amem',
         cache_correct cache cmem',
         refine_registers aregs cregs cmem' &
         refine_memory amem' cmem'].
 Proof.
   move=> Hcache Hregs Hmem Hget Hdec Hupd Hdec'.
   have Hget' := proj1 Hmem _ _ _ _ Hdec Hget.
-  have [amem' Hupd'] := PartMaps.upd_defined v'@t' Hget'.
-  have Hdec_eq := decode_monotonic _ Hget Hdec Hupd Hdec'.
-  exists amem'. split; trivial.
+  move: Hupd; rewrite /updm Hget Hget' /= => - [<-].
+  have Hdec_eq := decode_monotonic v' _ Hget Hdec Hdec'.
+  eexists; split; trivial.
   - move=> cmvec crvec Hlookup.
     case Hdec_pc: (decode _ _ _) => [pct|] //= Hpct_user.
     rewrite Hdec_eq in Hdec_pc.
     have := Hcache cmvec crvec Hlookup.
     rewrite Hdec_pc => /(_ Hpct_user) [ivec [ovec [Hdec_ivec Hdec_ovec Htrans]]].
-    rewrite -(decode_ivec_monotonic Hget Hdec Hupd Hdec') in Hdec_ivec.
-    rewrite -(decode_ovec_monotonic _ Hget Hdec Hupd Hdec') in Hdec_ovec.
+    rewrite -(decode_ivec_monotonic v' Hget Hdec Hdec') in Hdec_ivec.
+    rewrite -(decode_ovec_monotonic _ v' Hget Hdec Hdec') in Hdec_ovec.
     by eauto using And3.
   - split.
     + move=> w x ct'' st'' Hdec_ct' Hget''.
@@ -286,50 +267,43 @@ Proof.
   - split.
     + move=> w x ct'' st'' Hdec_ct' Hget''.
       rewrite Hdec_eq in Hdec_ct'.
+      move: Hget''; rewrite !getm_set.
       have [Heq|Hneq] := w =P addr.
-      * subst w.
-        rewrite (PartMaps.get_upd_eq Hupd) in Hget''.
-        rewrite (PartMaps.get_upd_eq Hupd').
-        case: Hget'' => ? ?. subst. congruence.
-      * rewrite (PartMaps.get_upd_neq Hneq Hupd) in Hget''.
-        rewrite (PartMaps.get_upd_neq Hneq Hupd').
-        by eapply (proj1 Hmem); eauto.
-    + move=> w x st Hget''.
-      have [Heq|Hneq] := w =P addr.
-      * subst w.
-        rewrite (PartMaps.get_upd_eq Hupd') in Hget''.
-        case: Hget'' => ? ?. subst x st.
-        exists ct'=> //.
-          by rewrite Hdec_eq.
-        by rewrite (PartMaps.get_upd_eq Hupd).
-      * rewrite (PartMaps.get_upd_neq Hneq Hupd') in Hget''.
-        have [ct'' Hdec_ct'' Hget_ct''] := proj2 Hmem _ _ _ Hget''.
-        rewrite -(PartMaps.get_upd_neq Hneq Hupd) in Hget_ct''.
-        rewrite -Hdec_eq in Hdec_ct''.
-        by eauto.
+      * subst w; move=> [? ?]; subst; congruence.
+      * by eapply (proj1 Hmem); eauto.
+    + move=> w x st Hget''; move: Hget'' Hdec_eq; rewrite /updm !getm_set.
+      have [_ {w}|Hneq] := altP (w =P addr).
+        move => [-> Ht]; eexists ct'=> //.
+        by rewrite Hdec_eq Hdec' Ht.
+      move=> Hget''.
+      have [ct'' Hdec_ct'' Hget_ct''] := proj2 Hmem _ _ _ Hget''.
+      rewrite Hget_ct''=> Hdec''; eexists ct''=> //.
+      by rewrite Hdec''.
 Qed.
 
 Lemma wf_entry_points_user_upd cmem cmem' addr v v' ct t ct' t' :
   wf_entry_points cmem ->
-  PartMaps.get cmem addr = Some v@ct ->
+  cmem addr = Some v@ct ->
   decode Symbolic.M cmem ct = Some (USER t) ->
-  PartMaps.upd cmem addr v'@ct' = Some cmem' ->
+  updm cmem addr v'@ct' = Some cmem' ->
   decode Symbolic.M cmem ct' = Some (USER t') ->
   wf_entry_points cmem'.
 Proof.
-  move=> Hwf Hget Hdec Hupd Hdec' addr' t''.
-  rewrite (PartMaps.get_upd Hupd) Hwf.
-  have [-> {addr'}|_] := altP (addr' =P addr).
-    by rewrite Hget (decode_monotonic _ Hget Hdec Hupd Hdec') Hdec Hdec' !andbF.
-  case: (PartMaps.get _ _) => [[i ti]|] //.
-  by rewrite (decode_monotonic _ Hget Hdec Hupd Hdec').
+move=> Hwf Hget Hdec Hupd Hdec' addr' t''; rewrite Hwf.
+have := decode_monotonic _ _ Hget Hdec Hdec'.
+move: Hupd; rewrite /updm Hget /= => - [<-] {cmem'} Hmono.
+rewrite getm_set.
+have [-> {addr'}|_] := altP (addr' =P addr).
+  by rewrite Hget !Hmono Hdec Hdec' !andbF.
+case: (cmem addr') => [[i ti]|] //.
+  by rewrite Hmono.
 Qed.
 
 Lemma mvec_in_kernel_user_upd cmem cmem' addr v v' ct t ct' t' :
   mvec_in_kernel cmem ->
-  PartMaps.get cmem addr = Some v@ct ->
+  cmem addr = Some v@ct ->
   decode Symbolic.M cmem ct = Some (USER t) ->
-  PartMaps.upd cmem addr v'@ct' = Some cmem' ->
+  updm cmem addr v'@ct' = Some cmem' ->
   decode Symbolic.M cmem ct' = Some (USER t') ->
   mvec_in_kernel cmem'.
 Proof.
@@ -340,45 +314,46 @@ Proof.
   { intros E. subst addr'.
     have CONTRA : Concrete.TKernel = ct by congruence. subst ct.
     by rewrite decode_kernel_tag in DEC. }
-  rewrite (PartMaps.get_upd_neq NEQ UPD).
-  eauto.
+  move: UPD; rewrite /updm GET /= => - [<-].
+  by rewrite getm_set (introF eqP NEQ) KER; eauto.
 Qed.
 
 Lemma mvec_in_kernel_kernel_upd cmem cmem' addr w :
   mvec_in_kernel cmem ->
-  PartMaps.upd cmem addr w@Concrete.TKernel = Some cmem' ->
+  updm cmem addr w@Concrete.TKernel = Some cmem' ->
   mvec_in_kernel cmem'.
 Proof.
-  intros MVEC UPD addr' IN.
-  have [?|/eqP NEQ] := altP (addr' =P addr); simpl in *; subst.
-  - erewrite PartMaps.get_upd_eq; eauto. now apply word_map_axioms.
-  - rewrite (PartMaps.get_upd_neq NEQ UPD).
-    now apply MVEC.
+intros MVEC UPD addr' IN.
+move: UPD; rewrite /updm; case: (cmem _) => //= _ [<-].
+rewrite getm_set.
+by have [?|/eqP NEQ] := altP (addr' =P addr); simpl in *; subst; eauto.
 Qed.
 
 Lemma refine_memory_upd' cache aregs cregs amem amem' cmem addr v ct t :
   cache_correct cache cmem ->
   refine_registers aregs cregs cmem ->
   refine_memory amem cmem ->
-  PartMaps.upd amem addr v@t = Some amem' ->
+  updm amem addr v@t = Some amem' ->
   decode Symbolic.M cmem ct = Some (USER t) ->
   exists cmem',
-    [/\ PartMaps.upd cmem addr v@ct = Some cmem',
+    [/\ updm cmem addr v@ct = Some cmem',
         cache_correct cache cmem',
         refine_registers aregs cregs cmem' &
         refine_memory amem' cmem' ].
 Proof.
   move=> Hcache Hregs Hmem Hupd Hdec.
-  have [[x t'] Hget] := PartMaps.upd_inv Hupd.
+  have [[x t'] Hget] : exists a, amem addr = Some a.
+    by move: Hupd; rewrite /updm; case: (amem _); eauto.
   have [ct' Hdec' Hget'] := proj2 Hmem _ _ _ Hget.
-  have [cmem' Hupd'] := PartMaps.upd_defined v@ct Hget'.
-  have Hdec_eq := decode_monotonic _ Hget' Hdec' Hupd' Hdec.
+  have Hupd' : updm cmem addr v@ct = Some (setm cmem addr v@ct).
+    by rewrite /updm Hget'.
+  have Hdec_eq := decode_monotonic v _ Hget' Hdec' Hdec.
   rewrite Hupd'. eexists. split; eauto.
   - move=> cmvec crvec Hlookup.
     rewrite Hdec_eq.
     move=> /(Hcache _ _ Hlookup) [ivec [ovec [Hdec_i Hdec_o Htrans]]].
-    rewrite -(decode_ivec_monotonic Hget' Hdec' Hupd' Hdec) in Hdec_i.
-    rewrite -(decode_ovec_monotonic _ Hget' Hdec' Hupd' Hdec) in Hdec_o.
+    rewrite -(decode_ivec_monotonic v Hget' Hdec' Hdec) in Hdec_i.
+    rewrite -(decode_ovec_monotonic _ v Hget' Hdec' Hdec) in Hdec_o.
     by eauto using And3.
   - split.
     + move=> r x'' ct'' st'' Hdec_ct'' Hget''.
@@ -387,15 +362,15 @@ Proof.
     + move=> r x'' st'' /(proj2 Hregs) [ct'' Hdec_ct'' Hget''].
       rewrite -Hdec_eq in Hdec_ct''.
       by eauto.
-  - split.
+  - move: Hupd; rewrite /updm Hget=> - [<-] {amem'}; split.
     + move=> w x'' ct'' st''.
-      rewrite Hdec_eq (PartMaps.get_upd Hupd) (PartMaps.get_upd Hupd').
+      rewrite Hdec_eq !getm_set.
       have [_ {w}|_] := altP (w =P addr).
         move=> Hdec_ct'' [Hv Hct]. move: Hv Hct Hdec_ct'' => <- <- {x'' ct''}.
         by rewrite Hdec; move => [->].
       by apply (proj1 Hmem).
     + move=> w x' st'.
-      rewrite (PartMaps.get_upd Hupd) (PartMaps.get_upd Hupd').
+      rewrite !getm_set.
       case: (w == addr) => [{w} [<- <-] {x' st'}|].
         exists ct=> //.
         by rewrite Hdec_eq.
@@ -406,52 +381,50 @@ Qed.
 
 Lemma refine_registers_upd areg creg creg' cmem r v v' ct t ct' t' :
   refine_registers areg creg cmem ->
-  PartMaps.get creg r = Some v@ct ->
+  creg r = Some v@ct ->
   decode Symbolic.R cmem ct = Some (USER t) ->
-  PartMaps.upd creg r v'@ct' = Some creg' ->
+  updm creg r v'@ct' = Some creg' ->
   decode Symbolic.R cmem ct' = Some (USER t') ->
   exists2 areg',
-    PartMaps.upd areg r v'@t' = Some areg' &
+    updm areg r v'@t' = Some areg' &
     refine_registers areg' creg' cmem.
 Proof.
   move=> Hregs Hget Hdec Hupd Hdec'.
   have Hget' := proj1 Hregs _ _ _ _ Hdec Hget.
-  have [areg' Hupd'] := PartMaps.upd_defined v'@t' Hget'.
-  exists areg'=> //. split.
+  have Hupd' : updm areg r v'@t' = Some (setm areg r v'@t').
+    by rewrite /updm Hget'.
+  move: Hupd; rewrite {1}/updm Hget /= => - [<-].
+  rewrite Hupd'; eexists => //; split.
   - move=> r' x ct'' st''.
-    rewrite (PartMaps.get_upd Hupd) (PartMaps.get_upd Hupd').
+    rewrite !getm_set.
     case: (r' == r) => [Hdec'' [Hx Hct'']|].
       move: Hx Hct'' Hdec'' => <- <-.
       by rewrite Hdec'=> [[->]].
     by apply (proj1 Hregs).
   - move=> r' x st''.
-    rewrite (PartMaps.get_upd Hupd) (PartMaps.get_upd Hupd').
+    rewrite !getm_set.
     case: (r' == r) => [[<- <-] {x st''}|]; first by eauto.
     by apply (proj2 Hregs).
 Qed.
 
 Lemma refine_registers_upd' areg areg' creg cmem r v ct t :
   refine_registers areg creg cmem ->
-  PartMaps.upd areg r v@t = Some areg' ->
+  updm areg r v@t = Some areg' ->
   decode _ cmem ct = Some (USER t) ->
   exists2 creg',
-    PartMaps.upd creg r v@ct = Some creg' &
+    updm creg r v@ct = Some creg' &
     refine_registers areg' creg' cmem.
 Proof.
-  move=> Hregs Hupd Hdec.
-  have [[v0 t0] Hget] := PartMaps.upd_inv Hupd.
+  rewrite /updm; case Hget: (areg r)=> [[v0 t0]|] //= Hregs [<-] Hdec.
   have [ct0 Hdec' Hget'] := proj2 Hregs _ _ _ Hget.
-  have [creg' Hupd'] := PartMaps.upd_defined v@ct Hget'.
-  exists creg'=> //.
-  split.
-  - move=> r' x ct' st'.
-    rewrite (PartMaps.get_upd Hupd) (PartMaps.get_upd Hupd').
+  rewrite Hget' /=.
+  eexists=> //; split.
+  - move=> r' x ct' st'; rewrite !getm_set.
     case: (r' == r) => [Hdec_ct' [Hx Hct']|].
       move: Hx Hct' Hdec_ct' => <- <- {x ct'}.
       by rewrite Hdec => [[<-]].
     by apply (proj1 Hregs).
-  - move=> r' x st'.
-    rewrite (PartMaps.get_upd Hupd) (PartMaps.get_upd Hupd').
+  - move=> r' x st'; rewrite !getm_set.
     case: (r' == r) => [[<- <-] {x st'}|]; first by rewrite -Hdec; eauto.
     by apply (proj2 Hregs).
 Qed.
@@ -495,11 +468,11 @@ Lemma analyze_cache cache cmem cmvec crvec op :
   cache_correct cache cmem ->
   Concrete.cache_lookup cache masks cmvec = Some crvec ->
   oapp (fun x => is_user x) false (decode Symbolic.P cmem (Concrete.ctpc cmvec)) ->
-  Concrete.cop cmvec = op_to_word op ->
+  Concrete.cop cmvec = mword_of_op op ->
   if Symbolic.privileged_op op then False else
   exists tpc : Symbolic.ttypes Symbolic.P, decode _ cmem (Concrete.ctpc cmvec) = Some (USER tpc) /\
   ((exists (ti : Symbolic.ttypes Symbolic.M)
-           (ts : hlist Symbolic.ttypes (Symbolic.inputs op))
+           (ts : hseq Symbolic.ttypes (Symbolic.inputs op))
            (rtpc : Symbolic.ttypes Symbolic.P)
            (rt : Symbolic.type_of_result Symbolic.ttypes (Symbolic.outputs op)),
     let ovec := Symbolic.mkOVec rtpc rt in
@@ -516,7 +489,7 @@ Proof.
   case: cmvec => op' tpc ti t1 t2 t3 /= CACHE LOOKUP INUSER EQ. subst op'.
   case: (CACHE _ crvec LOOKUP INUSER) =>
         [[op' tpc' ti' ts] /= [ovec /= [/decode_ivec_inv /= [E1|E1] E2 E3]]];
-  rewrite op_to_wordK in E1; last first.
+  rewrite mword_of_opK in E1; last first.
     case: E1 => [[?] ? -> ->]. subst op op'.
     move: E2 => /=.
     have [-> _| //] := (Concrete.ctrpc _ =P _).
@@ -529,7 +502,7 @@ Proof.
 Qed.
 
 Lemma miss_state_not_user st st' mvec :
-  Concrete.miss_state st mvec = Some st' ->
+  Concrete.miss_state st mvec = st' ->
   in_user st' ->
   False.
 Proof.
@@ -537,44 +510,15 @@ Proof.
   apply in_user_in_kernel in INUSER.
   unfold Concrete.miss_state in MISS.
   unfold in_kernel, Concrete.is_kernel_tag in INUSER.
-  by match_inv.
+  by rewrite -MISS /= eqxx in INUSER.
 Qed.
-
-(*
-(\* Need to double-check that is_true is not affecting the match below *\)
-Ltac analyze_cache :=
-  match goal with
-  | LOOKUP : Concrete.cache_lookup ?cache _ ?mvec = Some ?rvec,
-    PC     : PartMaps.get _ ?pc = Some ?i@_,
-    INST   : decode_instr ?i = Some _,
-    INUSER : in_user (Concrete.mkState _ _ _ ?pc@_ _),
-    CACHE  : cache_correct ?cache |- _ =>
-    unfold in_user in INUSER; simpl in INUSER;
-    assert (CACHEHIT := analyze_cache mvec CACHE LOOKUP INUSER (erefl _));
-    simpl in CACHEHIT;
-    repeat match type of CACHEHIT with
-    | exists _, _ => destruct CACHEHIT as [? CACHEHIT]
-    | _ /\ _ => destruct CACHEHIT as [? CACHEHIT]
-    | _ \/ _ => destruct CACHEHIT as [CACHEHIT | CACHEHIT]
-    | False => destruct CACHEHIT
-    end;
-    subst mvec; simpl in *; subst;
-    try match goal with
-    | H : context[decode (encode _)] |- _ =>
-      rewrite decodeK in H; simpl in *; subst
-    end
-  | MISS   : Concrete.miss_state _ _ = Some ?st',
-    INUSER : in_user ?st' |- _ =>
-    destruct (miss_state_not_user _ _ MISS INUSER)
-  end.
-*)
 
 Lemma valid_initial_user_instr_tags cst cst' v ti :
   cache_correct (Concrete.cache cst) (Concrete.mem cst) ->
   in_user cst ->
   in_user cst' ->
   Concrete.step _ masks cst cst' ->
-  PartMaps.get (Concrete.mem cst) (Concrete.pcv cst) = Some v@ti ->
+  Concrete.mem cst (Concrete.pcv cst) = Some v@ti ->
   oapp (fun x => is_user x) false (decode Symbolic.M (Concrete.mem cst) ti).
 Proof.
   move=> Hcache Huser Huser' Hstep Hget.
@@ -589,7 +533,7 @@ Proof.
     rewrite /in_user {}Hservice /= -{}Hpc_cst' => [[]].
     have [->|//] := (_ =P _).
     by rewrite decode_kernel_tag.
-  case: (Concrete.store_mvec _ _) => [cmem'|//] Hcst'.
+  rewrite /= => Hcst'.
   move: Huser'.
   by rewrite /in_user {}Hcst' /= decode_kernel_tag.
 Qed.
@@ -616,7 +560,7 @@ Proof.
         move=> E. rewrite -E in Hdec. by eauto.
       move/concrete.exec.stepP: Hstep Hcmvec Hdec_i Hdec_o.
       rewrite /step /build_cmvec {1}(Concrete.state_eta st) /=.
-      case Hget: (PartMaps.get _ (Concrete.pcv _)) => [[i cti]|] //=.
+      case Hget: (getm _ (Concrete.pcv _)) => [[i cti]|] //=.
       case Hdec_i: (decode_instr i) => [instr|] //=.
       destruct instr; move=> Hstep; match_inv; try by []; move => [?]; subst cmvec;
       unfold Concrete.next_state_reg, Concrete.next_state_pc,
@@ -629,14 +573,15 @@ Proof.
       repeat match goal with
       | H : Some _ = Some _ |- _ => inv H; simpl in *
       end; trivial.
-      rewrite /decode_ivec op_to_wordK /= => ?. match_inv.
+      rewrite /decode_ivec mword_of_opK /= => ?. match_inv.
       repeat match goal with
       | a : atom _ _ |- _ => destruct a; simpl in *
       | H : OP _ = OP _ |- _ => inv H
       end. simpl.
       move=> H /=.
-      match_inv.
-      by eapply decode_monotonic; eauto.
+      match_inv. rewrite hsheadE in Heqo3.
+      move: E1; rewrite /updm; case: (getm _ _) => /= [_|] // [<-].
+      eapply decode_monotonic; eauto. by eapply decode_monotonic; eauto.
     rewrite {}Hpc_st'.
     case=> _ Hop _ _.
     move: ovec {Htrans} Hdec_o.
