symbolic/symbolic.v
@@ -1,8 +1,5 @@
-Require Import Arith ZArith.
-Require Import Coq.Bool.Bool.
-Require Coq.Vectors.Vector.
-
 Require Import ssreflect ssrfun ssrbool eqtype ssrnat seq.
+Require Import hseq word partmap.
 
 Require Import lib.utils common.common.
 Require Import lib.ssr_list_utils.
@@ -20,6 +17,19 @@ Module Symbolic.
        we probably don't want to do that. *)
 
 Inductive tag_kind : Type := R | M | P.
+
+Module Import TagKindEq.
+Definition tag_kind_eq (tk1 tk2 : tag_kind) : bool :=
+  match tk1, tk2 with
+  | R, R | M, M | P, P => true | _, _ => false
+  end.
+
+Lemma tag_kind_eqP : Equality.axiom tag_kind_eq.
+Proof. by do !case; constructor. Qed.
+
+Definition tag_kind_eqMixin := EqMixin tag_kind_eqP.
+Canonical tag_kind_eqType := Eval hnf in EqType tag_kind tag_kind_eqMixin.
+End TagKindEq.
 
 Definition inputs (op : opcode) : seq tag_kind :=
   match op with
@@ -84,13 +94,13 @@ Record IVec : Type := mkIVec {
   op  : vopcode;
   tpc : tag_type P;
   ti  : tag_type M;
-  ts  : hlist tag_type (vinputs op)
+  ts  : hseq tag_type (vinputs op)
 }.
 
 Lemma ivec_eq_inv op op' tpc tpc' ti ti' ts ts'
                   (p : mkIVec op tpc ti ts = mkIVec op' tpc' ti' ts') :
   [/\ op = op', tpc = tpc', ti = ti' &
-      existT (hlist tag_type \o vinputs) op ts = existT _ op' ts'].
+      existT (hseq tag_type \o vinputs) op ts = existT _ op' ts'].
 Proof. inversion p. by constructor. Qed.
 
 Definition type_of_result (o : option tag_kind) :=
@@ -119,8 +129,6 @@ Section WithClasses.
 Context (t : machine_types)
         {ops : machine_ops t}.
 
-Import PartMaps.
-
 Class params := {
   ttypes :> tag_kind -> eqType;
 
@@ -133,12 +141,12 @@ Context {sp : params}.
 
 Open Scope word_scope.
 
-Local Notation word := (word t).
+Local Notation word := (mword t).
 Let atom := (atom word).
-Local Notation "x .+1" := (Word.add x Word.one).
+Local Notation "x .+1" := (x + 1).
 
-Local Notation memory := (word_map t (atom (ttypes M))).
-Local Notation registers := (reg_map t (atom (ttypes R))).
+Local Notation memory := {partmap word -> atom (ttypes M)}.
+Local Notation registers := {partmap reg t -> atom (ttypes R)}.
 
 Record state := State {
   mem : memory;
@@ -168,7 +176,7 @@ Definition get_syscall (addr : word) : option syscall :=
   ofind (fun sc => address sc == addr) table.
 
 Definition run_syscall (sc : syscall) (st : state) : option state :=
-  match transfer (mkIVec SERVICE (common.tag (pc st)) (entry_tag sc) tt) with
+  match transfer (mkIVec SERVICE (common.tag (pc st)) (entry_tag sc) [hseq of [::]]) with
   | Some _ => sem sc st
   | None => None
   end.
@@ -185,7 +193,7 @@ Definition next_state_reg_and_pc (st : state) (iv : @IVec ttypes)
     | OP op => fun ov =>
       match outputs op as o return (type_of_result _ o -> option state) with
         | Some R => fun tr' =>
-            do! regs' <- upd (regs st) r x@tr';
+            do! regs' <- updm (regs st) r x@tr';
             Some (State (mem st) regs' pc'@(trpc ov) (internal st))
         | _ => fun _ => None
       end (tr ov)
@@ -206,95 +214,93 @@ Definition next_state_pc (st : state) (iv : @IVec ttypes)
     end
   ).
 
-Import HListNotations.
-
 Inductive step (st st' : state) : Prop :=
 | step_nop : forall mem reg pc tpc i ti extra
     (ST   : st = State mem reg pc@tpc extra)
-    (PC   : get mem pc = Some i@ti)
+    (PC   : mem pc = Some i@ti)
     (INST : decode_instr i = Some (Nop _)),
-    let mvec := mkIVec NOP tpc ti [hl] in forall
+    let mvec := mkIVec NOP tpc ti [hseq] in forall
     (NEXT : next_state_pc st mvec (pc.+1) = Some st'),    step st st'
-| step_const : forall mem reg pc tpc i ti n r old told extra
+| step_const : forall mem reg pc tpc i ti n r old (told : ttypes R) extra
     (ST   : st = State mem reg pc@tpc extra)
-    (PC   : get mem pc = Some i@ti)
+    (PC   : mem pc = Some i@ti)
     (INST : decode_instr i = Some (Const n r))
-    (OLD  : get reg r = Some old@told),
-    let mvec := mkIVec CONST tpc ti [hl told] in forall
-    (NEXT : next_state_reg st mvec r (Word.casts n) = Some st'),   step st st'
+    (OLD  : reg r = Some old@told),
+    let mvec := mkIVec CONST tpc ti [hseq : ttypes of told] in forall
+    (NEXT : next_state_reg st mvec r (swcast n) = Some st'),   step st st'
 | step_mov : forall mem reg pc tpc i ti r1 w1 t1 r2 old told extra
     (ST   : st = State mem reg pc@tpc extra)
-    (PC   : get mem pc = Some i@ti)
+    (PC   : mem pc = Some i@ti)
     (INST : decode_instr i = Some (Mov r1 r2))
-    (R1W  : get reg r1 = Some w1@t1)
-    (OLD  : get reg r2 = Some old@told),
-    let mvec := mkIVec MOV tpc ti [hl t1; told] in forall
+    (R1W  : reg r1 = Some w1@t1)
+    (OLD  : reg r2 = Some old@told),
+    let mvec := mkIVec MOV tpc ti [hseq : ttypes of t1; told] in forall
     (NEXT : next_state_reg st mvec r2 w1 = Some st'),   step st st'
 | step_binop : forall mem reg pc tpc i ti op r1 r2 r3 w1 w2 t1 t2 old told extra
     (ST   : st = State mem reg pc@tpc extra)
-    (PC   : get mem pc = Some i@ti)
+    (PC   : mem pc = Some i@ti)
     (INST : decode_instr i = Some (Binop op r1 r2 r3))
-    (R1W  : get reg r1 = Some w1@t1)
-    (R2W  : get reg r2 = Some w2@t2)
-    (OLD  : get reg r3 = Some old@told),
-    let mvec := mkIVec (BINOP op) tpc ti [hl t1; t2; told] in forall
+    (R1W  : reg r1 = Some w1@t1)
+    (R2W  : reg r2 = Some w2@t2)
+    (OLD  : reg r3 = Some old@told),
+    let mvec := mkIVec (BINOP op) tpc ti [hseq : ttypes of t1; t2; told] in forall
     (NEXT : next_state_reg st mvec r3 (binop_denote op w1 w2) = Some st'),
       step st st'
 | step_load : forall mem reg pc tpc i ti r1 r2 w1 w2 t1 t2 old told extra
     (ST   : st = State mem reg pc@tpc extra)
-    (PC   : get mem pc = Some i@ti)
+    (PC   : mem pc = Some i@ti)
     (INST : decode_instr i = Some (Load r1 r2))
-    (R1W  : get reg r1 = Some w1@t1)
-    (MEM1 : get mem w1 = Some w2@t2)
-    (OLD  : get reg r2 = Some old@told),
-    let mvec := mkIVec LOAD tpc ti [hl t1; t2; told] in forall
+    (R1W  : reg r1 = Some w1@t1)
+    (MEM1 : mem w1 = Some w2@t2)
+    (OLD  : reg r2 = Some old@told),
+    let mvec := mkIVec LOAD tpc ti [hseq : ttypes of t1; t2; told] in forall
     (NEXT : next_state_reg st mvec r2 w2 = Some st'),    step st st'
 | step_store : forall mem reg pc i r1 r2 w1 w2 tpc ti t1 t2 old told extra
     (ST   : st = State mem reg pc@tpc extra)
-    (PC   : get mem pc = Some i@ti)
+    (PC   : mem pc = Some i@ti)
     (INST : decode_instr i = Some (Store r1 r2))
-    (R1W  : get reg r1 = Some w1@t1)
-    (R2W  : get reg r2 = Some w2@t2)
-    (OLD  : get mem w1 = Some old@told),
-    let mvec := mkIVec STORE tpc ti [hl t1; t2; told] in forall
+    (R1W  : reg r1 = Some w1@t1)
+    (R2W  : reg r2 = Some w2@t2)
+    (OLD  : mem w1 = Some old@told),
+    let mvec := mkIVec STORE tpc ti [hseq : ttypes of t1; t2; told] in forall
     (NEXT : next_state st mvec (fun ov =>
-                 do! mem' <- upd mem w1 w2@(tr ov);
+                 do! mem' <- updm mem w1 w2@(tr ov);
                  Some (State mem' reg (pc.+1)@(trpc ov) extra)) = Some st'),
               step st st'
 | step_jump : forall mem reg pc i r w tpc ti t1 extra
     (ST   : st = State mem reg pc@tpc extra)
-    (PC   : get mem pc = Some i@ti)
+    (PC   : mem pc = Some i@ti)
     (INST : decode_instr i = Some (Jump r))
-    (RW   : get reg r = Some w@t1),
-    let mvec := mkIVec JUMP tpc ti [hl t1] in forall
+    (RW   : reg r = Some w@t1),
+    let mvec := mkIVec JUMP tpc ti [hseq : ttypes of t1] in forall
     (NEXT : next_state_pc st mvec w = Some st'),    step st st'
 | step_bnz : forall mem reg pc i r n w tpc ti t1 extra
     (ST   : st = State mem reg pc@tpc extra)
-    (PC   : get mem pc = Some i@ti)
+    (PC   : mem pc = Some i@ti)
     (INST : decode_instr i = Some (Bnz r n))
-    (RW   : get reg r = Some w@t1),
-     let mvec := mkIVec BNZ tpc ti [hl t1] in
-     let pc' := Word.add pc (if w == Word.zero
-                             then Word.one else Word.casts n) in forall
+    (RW   : reg r = Some w@t1),
+     let mvec := mkIVec BNZ tpc ti [hseq : ttypes of t1] in
+     let pc' := pc + (if w == 0%w
+                      then 1%w else swcast n) in forall
     (NEXT : next_state_pc st mvec pc' = Some st'),     step st st'
 | step_jal : forall mem reg pc i r w tpc ti t1 old told extra
     (ST : st = State mem reg pc@tpc extra)
-    (PC : get mem pc = Some i@ti)
+    (PC : mem pc = Some i@ti)
     (INST : decode_instr i = Some (Jal r))
-    (RW : get reg r = Some w@t1)
-    (OLD : get reg ra = Some old@told),
-     let mvec := mkIVec JAL tpc ti [hl t1; told] in forall
+    (RW : reg r = Some w@t1)
+    (OLD : reg ra = Some old@told),
+     let mvec := mkIVec JAL tpc ti [hseq : ttypes of t1; told] in forall
     (NEXT : next_state_reg_and_pc st mvec ra (pc.+1) w = Some st'), step st st'
 | step_syscall : forall mem reg pc sc tpc extra
     (ST : st = State mem reg pc@tpc extra)
-    (PC : get mem pc = None)
+    (PC : mem pc = None)
     (GETCALL : get_syscall pc = Some sc)
     (CALL : run_syscall sc st = Some st'), step st st'.
 
 End WithClasses.
 
-Notation memory t s := (word_map t (atom (word t) (@ttypes s M))).
-Notation registers t s := (reg_map t (atom (word t) (@ttypes s R))).
+Notation memory t s := {partmap mword t -> atom (mword t) (@ttypes s M)}.
+Notation registers t s := {partmap reg t -> atom (mword t) (@ttypes s R)}.
 
 End Symbolic.
 
@@ -318,6 +324,8 @@ Qed.
 
 Definition state_eqMixin mt p := EqMixin (@state_eqbP mt p).
 Canonical state_eqType mt p := Eval hnf in EqType _ (@state_eqMixin mt p).
+
+Export TagKindEq.
 
 End Exports.
 
