compartmentalization/isolate_sets.v
@@ -1,13 +1,11 @@
-Require Import List ZArith Arith Sorted Bool.
-
-Require Import ssreflect ssrfun ssrbool eqtype ssrnat seq fintype finset.
+Require Import ssreflect ssrfun ssrbool eqtype ssrnat seq fintype finset ssrint.
+Require Import word partmap.
 
 Require Import lib.utils common.common.
 Require Import compartmentalization.ranges.
 
 Set Bullet Behavior "Strict Subproofs".
 Import DoNotation.
-Import PartMaps.
 
 Generalizable All Variables.
 
@@ -16,31 +14,30 @@ Section WithClasses.
 Context  {t            : machine_types}
          {ops          : machine_ops t}
          {spec         : machine_ops_spec ops}
-        `{pm           : partial_map Map (word t)}
          {V            : Type}
-         (to_word      : V -> word t).
+         (to_word      : V -> mword t).
 
 Open Scope word_scope.
 
-Definition isolate_get_range (M : Map V) (p : word t) : option {set (word t)} :=
-  do! low  <- get M p;
-  do! high <- get M (p + 1);
-  Some [set i : word t in range (to_word low) (to_word high)].
+Definition isolate_get_range (m : {partmap mword t -> V}) (p : mword t) : option {set (mword t)} :=
+  do! low  <- m p;
+  do! high <- m (p + 1);
+  Some [set i : mword t in range (to_word low) (to_word high)].
 
-Fixpoint isolate_get_ranges (M : Map V)
-                            (p : word t)
-                            (n : nat) : option {set (word t)} :=
+Fixpoint isolate_get_ranges (m : {partmap mword t -> V})
+                            (p : mword t)
+                            (n : nat) : option {set (mword t)} :=
   match n with
     | O    => Some set0
-    | S n' => do! here <- isolate_get_range M p;
-              do! rest <- isolate_get_ranges M (p + 2) n';
+    | S n' => do! here <- isolate_get_range m p;
+              do! rest <- isolate_get_ranges m (p + as_word 2) n';
               Some (here :|: rest)
   end.
 
-Definition isolate_create_set (M : Map V)
-                              (base : word t) : option {set (word t)} :=
-  do! pairs <- get M base;
-  isolate_get_ranges M (base + 1) (Z.to_nat (Word.signed (to_word pairs))).
+Definition isolate_create_set (m : {partmap mword t -> V})
+                              (base : mword t) : option {set (mword t)} :=
+  do! pairs <- m base;
+  isolate_get_ranges m (base + 1) (eqtype.val (to_word pairs)).
 
 Local Notation "x ?= y" := (x = Some y) (at level 70, no associativity).
 
